Test/IO/types.mlir
@@ -1,0 +1,18 @@
+// RUN: VEIR_ROUNDTRIP
+
+"builtin.module"() ({
+  "func.func"() <{function_type = (!io.address) -> (), sym_name = "main"}> ({
+    ^bb0(%arg0: !io.address):
+      %0 = "test.test"() : () -> !io.address
+      "func.return"() : () -> ()
+  }) : () -> ()
+}) : () -> ()
+
+// CHECK:      "builtin.module"() ({
+// CHECK-NEXT:   ^{{.*}}():
+// CHECK-NEXT:     "func.func"() <{"function_type" = (!io.address) -> (), "sym_name" = "main"}> ({
+// CHECK-NEXT:       ^{{.*}}(%{{.*}} : !io.address):
+// CHECK-NEXT:         %{{.*}} = "test.test"() : () -> !io.address
+// CHECK-NEXT:         "func.return"() : () -> ()
+// CHECK-NEXT:     }) : () -> ()
+// CHECK-NEXT: }) : () -> ()
